

# Logarithmic differentiation (LD) - Solutions

**Problem 1** (a) Write as an exponential with base 5.  $7^{3x}$ .

**Solution:**  $7 = 5^{\log_5(7)}$ , so

$$7^{3x} = \left(5^{\log_5(7)}\right)^{3x} = 5^{3x \log_5(7)}$$

(b) Write in terms of the natural logarithm.  $\log_3(4)$ .

**Solution:** The change of base formula says  $\log_a(u) = \frac{\log_b(u)}{\log_b(a)}$ , so

$$\log_3(4) = \frac{\ln(4)}{\ln(3)}$$

(c) Expand the following:  $\log_{1/2} \left( \frac{6x^5(2 + \tan(x))^x}{\sqrt[5]{e^{4x} + 1}} \right)$ .

**Solution:**

$$\log_{1/2} \left( \frac{6x^5(2 + \tan(x))^x}{\sqrt[5]{e^{4x} + 1}} \right) = \log_{1/2}(6) + 5 \log_{1/2}(x) + x \log_{1/2}(2 + \tan(x)) - \frac{1}{5} \log_{1/2}(e^{4x} + 1)$$

---

**Problem 2** Find all real numbers  $x$  which satisfy each of the following equations.

(a)  $\log_x(25) = 2$ .

**Solution:** Recall that, by definition of the inverse to an exponential function,

$$\log_b(x) = y \iff x = b^y.$$

Using this relationship we have  $\log_x(25) = 2 \iff x^2 = 25$ . Therefore

$$\begin{aligned} x^2 = 25 &\implies x = \pm 5, \\ &\implies x = 5 \quad (\text{base of log is always } > 0). \end{aligned}$$

Therefore  $x = 5$  is the only solution to  $\log_x(25) = 2$ .

(b)  $7^x = 15$

**Solution:** Similar to the previous problem,

$$\log_b(x) = y \iff x = b^y.$$

Using this relationship we have  $7^x = 15 \iff x = \log_7(15)$ . Therefore  $x = \log_7(15)$  is the only solution to  $7^x = 15$ .

(c)  $\ln(x) + 1 = 0$ .

**Solution:** Similar to the previous two problems we'll use the relationship

$$\ln(x) = y \iff x = e^y.$$

Before applying this relationship we perform a bit of algebra first:

$$\ln(x) + 1 = 0 \implies \ln(x) = -1.$$

Now we have  $\ln(x) = -1 \iff x = e^{-1}$ . Therefore  $x = e^{-1} (= 1/e)$  is the only solution to  $\ln(x) + 1 = 0$ .

---

**Problem 3** True or False:

(1) If  $f(x) = (x - 2)^x$ , then  $f'(x) = x(x - 2)^{x-1}$ .

**Solution:** False. Any time that you have a function of  $x$  raised to a function of  $x$ , in order to compute the derivative you need to use logarithmic differentiation (or something equivalent).

Correct derivative of  $f$ :

$$\begin{aligned} f(x) &= (x - 2)^x \implies f(x) = e^{x \ln(x-2)} \\ \implies f'(x) &= e^{x \ln(x-2)} \cdot \left( 1 \cdot \ln(x-2) + x \cdot \frac{1}{x-2} \right) \\ \implies f'(x) &= (x - 2)^x \cdot \left( \ln(x-2) + \frac{x}{x-2} \right) \end{aligned}$$

(2) If  $f(x) = (3x)^x$ , then  $f'(x) = (3x)^x \ln(3x)$ .

**Solution:** False. Same as part (1).

Correct derivative of  $f$ :

$$\begin{aligned} f(x) &= (3x)^x \implies f(x) = e^{x \cdot \ln(3x)} \\ \implies f'(x) &= e^{x \cdot \ln(3x)} \left( 1 \cdot \ln(3x) + x \cdot \frac{3}{3x} \right) \\ \implies f'(x) &= (3x)^x (\ln(3x) + 1) \end{aligned}$$

---

**Problem 4** Find the derivatives of the following functions:

(a)  $f(x) = x^{e^x} + 7x$

**Solution:**  $f'(x) = \frac{d}{dx} (x^{e^x}) + \frac{d}{dx} (7x) = \frac{d}{dx} (x^{e^x}) + 7$ . So the real problem is to find  $\frac{d}{dx} (x^{e^x})$ .

We will use logarithmic differentiation.

First, we take natural logarithm of both sides of the equation  $g(x) = x^{e^x}$ .

$$\ln(g(x)) = e^x \ln(x).$$

Now, we differentiate both sides.

$$\frac{g'(x)}{g(x)} = e^x \ln(x) + \frac{e^x}{x}.$$

Next, we solve for  $g'(x)$ .

$$g'(x) = g(x) \left( e^x \ln(x) + \frac{e^x}{x} \right).$$

Now, we substitute.

$$g'(x) = x^{e^x} \left( e^x \ln(x) + \frac{e^x}{x} \right).$$

ALTERNATIVE APPROACH

$$\begin{aligned} \frac{d}{dx} (x^{e^x}) &= \frac{d}{dx} (e^{\ln(x)e^x}) \\ &= \frac{d}{dx} (e^{e^x \ln(x)}) \\ &= e^{e^x \ln(x)} \left( e^x \ln(x) + \frac{e^x}{x} \right) \\ &= x^{e^x} \left( e^x \ln(x) + \frac{e^x}{x} \right). \end{aligned}$$

$$\text{Thus, } f'(x) = x^{e^x} \left( e^x \ln(x) + \frac{e^x}{x} \right) + 7.$$

(b)  $g(x) = (\ln(x) + 9)^{\sec(x^4)}$

**Solution:** We will use logarithmic differentiation.

First, we take natural logarithm .

$$\ln(g(x)) = \sec(x^4) \ln(\ln(x) + 9)$$

Then, we differentiate.

$$\frac{g'(x)}{g(x)} = \sec(x^4) \tan(x^4) 4x^3 \ln(\ln(x) + 9) + \frac{\sec(x^4)}{x(\ln(x) + 9)}$$

We multiply by  $g(x)$ .

$$g'(x) = g(x) \left( 4x^3 \sec(x^4) \tan(x^4) \ln(\ln(x) + 9) + \frac{\sec(x^4)}{x(\ln(x) + 9)} \right)$$

We substitute.

$$g'(x) = (\ln(x) + 9)^{\sec(x^4)} \left( 4x^3 \sec(x^4) \tan(x^4) \ln(\ln(x) + 9) + \frac{\sec(x^4)}{x(\ln(x) + 9)} \right)$$

ALTERNATIVE APPROACH

$$\begin{aligned}
g'(x) &= \frac{d}{dx} \left( (\ln(x) + 9)^{\sec(x^4)} \right) \\
&= \frac{d}{dx} \left( e^{\sec(x^4) \ln(\ln(x) + 9)} \right) \\
&= e^{\sec(x^4) \ln(\ln(x) + 9)} \left( 4x^3 \sec(x^4) \tan(x^4) \ln(\ln(x) + 9) + \sec(x^4) \frac{\frac{1}{x}}{\ln(x) + 9} \right) \\
&= (\ln(x) + 9)^{\sec(x^4)} \left( 4x^3 \sec(x^4) \tan(x^4) \ln(\ln(x) + 9) + \frac{\sec(x^4)}{x(\ln(x) + 9)} \right).
\end{aligned}$$

(c)  $f(x) = \frac{(x+1)^5(\sin(x)+5)^4}{(x^2+5)\sqrt{x-3}}$

**Solution:**

$$\begin{aligned}
\ln(f(x)) &= \ln(x+1)^5 + \ln(\sin(x)+5)^4 - \ln(x^2+5) - \ln\sqrt{x-3} \\
&= 5\ln(x+1) + 4\ln(\sin(x)+5) - \ln(x^2+5) - \frac{1}{2}\ln(x-3)
\end{aligned}$$

Now we differentiate.

$$\frac{f'(x)}{f(x)} = \frac{5}{x+1} + \frac{4\cos(x)}{\sin(x)+5} - \frac{2x}{x^2+5} - \frac{1}{2(x-3)}$$

Then we solve for  $f'(x)$ .

$$f'(x) = f(x) \left( \frac{5}{x+1} + \frac{4\cos(x)}{\sin(x)+5} - \frac{2x}{x^2+5} - \frac{1}{2(x-3)} \right) \text{ Then we substitute.}$$

$$f'(x) = \frac{(x+1)^5(\sin(x)+5)^4}{(x^2+5)\sqrt{x-3}} \left( \frac{5}{x+1} + \frac{4\cos(x)}{\sin(x)+5} - \frac{2x}{x^2+5} - \frac{1}{2(x-3)} \right)$$

(d)  $h(x) = \frac{(x^2-7)^5}{\cos^7(x^2-5)}$

**Solution:** Since  $h(x)$  changes sign on its domain, we write :

$$\begin{aligned}
\ln|h(x)| &= \ln \left( \frac{|x^2-7|^5}{|\cos^7(x^2-5)|} \right) \\
&= 5 \cdot \ln(|x^2-7|) - 7 \cdot \ln(|\cos(x^2-5)|)
\end{aligned}$$

Differentiate both sides with respect to  $x$ , (explanation given on the next page):

$$\frac{h'(x)}{h(x)} = 5 \frac{2x}{x^2-7} - 7 \frac{-\sin(x^2-5)2x}{\cos(x^2-5)}$$

$$h'(x) = h(x) \left( 5 \frac{2x}{x^2-7} - 7 \frac{-\sin(x^2-5)2x}{\cos(x^2-5)} \right) =$$

$$= \frac{(x^2-7)^5}{\cos^7(x^2-5)} \left( \frac{10x}{x^2-7} + \frac{14x \sin(x^2-5)}{\cos(x^2-5)} \right) =$$

$$= \frac{(x^2 - 7)^4}{\cos^7(x^2 - 5)} (10x + 14x(x^2 - 7) \tan(x^2 - 5))$$

*EXPLANATION: The function  $h(x)$  assumes negative values on some intervals. On those intervals*

$$(\ln(|h(x)|))' = (\ln(-h(x)))' = \frac{-h'(x)}{-h(x)} = \frac{h'(x)}{h(x)},$$

*Also, e.g., if  $x^2 - 7 < 0$*

$$(\ln(|x^2 - 7|))' = (\ln(-(x^2 - 7)))' = \frac{-2x}{-(x^2 - 7)} = \frac{2x}{x^2 - 7} .$$


---